We now use \emph{countdown} to define the inverse
hyperoperation hierarchy, which features elegant new definitions of
division, $\log$, and $\log^{*}$.
We then modify the inverse hyperoperation hierarchy to arrive at the inverse
Ackermann hierarchy.

\subsection{The inverse hyperoperations, including \li{div}, \li{log}, and \li{log*}}

\begin{defn} \label{defn: inv-hyperop}
	The inverse hyperoperations, written $a\angle{n}b$, are defined as:
	\begin{equation}
	a\angle{n}b \; \triangleq \; \begin{cases}
	b - 1 & \hspace{-10pt} \quad \text{ if } n = 0 \\
	\cdt{a\angle{n-1}}{a_n}(b) & \hspace{-10pt} \quad \text{ if } n \ge 1
	\end{cases}
	\ \ \quad \text{ where } \ a_n = \begin{cases}
	a & \hspace{-10pt}\text{ if } n = 1 \\
	0 & \hspace{-10pt}\text{ if } n = 2 \\
	1 & \hspace{-10pt}\text{ if } n \ge 3
	\end{cases}
	\end{equation}
\begin{lstlisting}
`\href{https://github.com/inv-ack/inv-ack/blob/6099297c6ab0e16d14b037fb5ed600c4d22818f6/applications.v#L23-L28}{Fixpoint inv\_hyperop}` (a n b : nat) : nat :=
  match n with
  | 0 => b - 1
  | S n' => countdown_to (hyperop_init a n') (inv_hyperop a n') b
  end.
\end{lstlisting}
\end{defn}
\hide{
Continuing with the notion of upper-inverses we have used thus far,
we aim for the \emph{ceiling} of division and $\log$ on real numbers, $\left\lceil b/a \right\rceil$ and $\left\lceil \log_ab \right\rceil$. The iterated logarithm is formally defined as the minimum number of times $\log$ needs to be iteratively
applied to the input for the result to become less than or equal to $1$.
Thus it is natural to define it using \emph{countdown}.

\begin{defn} \label{defn: divc} \label{defn: logc} \label{defn: log*}
\[
\divc(a, b) \! \triangleq \! \cdt{\left(\lambda b. (b{-}a)\right)}{0}(b) \quad
\logc(a, b) \! \triangleq \! \cdt{\left(\lambda b. \divc(a, b)\right)}{1}(b) \quad
\log^*(a, b) \! \triangleq \! \cdt{\left(\lambda b. \logc(a, b)\right)}{1}(b)
%\begin{array}{c}
%\divc(a, b) \triangleq \cdt{\left(\lambda b. (b-a)\right)}{0}(b) \qquad
%\logc(a, b) \triangleq \cdt{\left(\lambda b. \divc(a, b)\right)}{1}(b) \\
%\log^*(a, b) \triangleq \cdt{\left(\lambda b. \logc(a, b)\right)}{1}(b)
%\end{array}
\]
\begin{lstlisting}
Definition divc a b := countdown_to 0 (fun n => n - a) b.
Definition logc a b := countdown_to 1 (divc a) b.
Definition logstar a b := countdown_to 1 (logc a) b.
\end{lstlisting}\vspace*{-0.5\baselineskip}
\end{defn}
}%end hide
\hide{Proving $\forall a, b \ge 1,~\divc(a, b) = \left\lceil b/a \right\rceil$ serves
to prove that all three definitions are correct, since that statement implies
the correctness of  $\logc$, which in turn implies the correctness of $\log^*$. We will prove this in \ref{blah},
together with the correctness of the entire hyperoperation hierarchy.
}
where the Curried $a\angle{n{-}1}$ denotes the single-variable function 
$\lambda b.a\angle{n{-}1}b$.
We now show that $a\angle{n}$ is the inverse to $a[n]$. 
First note that $a\angle{0}\in \contract_0$.~Then:
\begin{lem}
$a\angle{1}b = b - a$.
\end{lem}
\begin{proof}
Since $a\angle{0} \in \contract_0 \subseteq \contract_{a}$, Theorem~\ref{thm: cdt-recursion} applies.
\begin{equation*}
a\angle{1}b \quad = \quad \cdt{\left(a\angle{0}\right)}{a}(b) \quad = \quad \begin{cases}
0 & \text{ if } b\le a \\ 1 + a\angle{1}(b - 1) & \text{ if } b\ge a+1 \end{cases} \\
\end{equation*}
Then, $a\angle{1}b = b - a$ by induction on $b$.
\end{proof}
\begin{col} \label{col: inv-hyperop-1-contr1}
$\forall a \ge 1, a\angle{1} \in \contract_1$.
\end{col}
\hide{\begin{col} \label{col: inv-hyperop-234}
{\color{magenta}$\forall a \in \mathbb{N}$}:
 {\color{blue} For all $a \in \mathbb{N}$},
\begin{enumerate}
	\item If $a\ge 1$, $a\angle{2}b = \divc(a, b) \ \forall b$.
	\item If $a\ge 2$, $a\angle{3}b = \logc(a, b) \ \forall b$ and $a\angle{4}b = \logstarc(a, b) \ \forall b$.
\end{enumerate}
\end{col}}%end hide
%Now we are ready to prove the correctness of the inverse hyperoperations.
Note: $a\angle{n}b$ is a total function, but it is never actually used for $a = 0$ when $n \ge 2$ or for $a=1$ when $n \ge 3$. For the values
we do care about, we have our inverse:
\begin{thm} \label{thm: inv-hyperop-correct}
When $n\le 1$, or $n \le 2 \wedge a\ge 1$, or $a\ge 2$, then
$a\angle{n} = \left(a[n]\right)^{-1}_+$.
\end{thm}
\begin{proof}
$\forall n \ge 2,~$ let $a_0 = a, a_1 = 0, a_n = 1$. Then define
\begin{equation*}
P(n) \triangleq  \Big(a[n] \in \repeatable_{a_n}\Big)\ \text{ and } \
Q(n) \triangleq  \Big((a\angle{n} = \left(a[n]\right)^{-1}_+ \Big)
\end{equation*}
We have three goals:
(1) $\forall a.~ Q(0) \wedge Q(1)$.
(2) $\forall a \ge 1.~ Q(2)$.
(3) $\forall a \ge 2.~ Q(n)$. \\
Note that \mbox{$\forall n.~ a\angle{n+1}$} $= \cdt{a\angle{n}}{a_n}$ and $a[n+1] = \rf{a[n]}{a_n}$. By Theorem~\ref{thm: cdt-inv-rf},

\vspace*{-1em}
\noindent\begin{minipage}{.45\linewidth}
\begin{equation}
P(n) \Rightarrow Q(n) \Rightarrow Q(n+1) \label{eq: tmp-induction-1}
\end{equation}
\end{minipage}
\begin{minipage}{.55\linewidth}
\begin{equation}
\qquad a_{n} \ge 1 \Rightarrow P(n) \Rightarrow P(n+1) \label{eq: tmp-induction-2}
\end{equation}
\end{minipage}
Goal 1: $P(0) \iff \lambda b.(b+1)\in \repeatable_a$ and
$Q(0) \iff a\angle{0} = \left(a[0]\right)^{-1} \iff (b-~1\le c \iff b\le c+1)$.
These are both straightforward, and $Q(1)$ holds by~(\ref{eq: tmp-induction-1}). Goal 2: we have $a \ge 1$, so
$P(1)$ holds by $P(0)$ and~(\ref{eq: tmp-induction-2}), and 
$Q(2)$ holds by $Q(1)$ and~(\ref{eq: tmp-induction-1}).
Goal 3: we have $a\ge 2$, and using~(\ref{eq: tmp-induction-1}) and $Q(0)$
reduces the goal to $P(n)$. Using~(\ref{eq: tmp-induction-2}) and the fact that $\forall n \neq 1.~a_n\ge 1$, the goal reduces to $P(2)$. This unfolds to:
\begin{equation*}
a[2]\in \repeatable_0 \iff \forall b < c.~ab < ac \quad \wedge \quad \forall b \ge 1.~ab \ge b+1\text{,}
\end{equation*}
which is straightforward for $a\ge 2$. Induction on n gives us the third goal.
\end{proof}
%With this theorem, we have proved the correctness of $\divc$, $\logc$ and $\log^*$, as well as the whole inverse hyperoperation hierarchy.
\begin{rem}
Three early hyperoperations are $a[2]b = ab$, $a[3]b = a^b$ and \linebreak $a[4]b = \! ^ba$, so, by Theorem~\ref{thm: inv-hyperop-correct}, we can define their inverses $\left\lceil b/a \right\rceil$, $\left\lceil \log_a b \right\rceil$, and $\log^*_a b$ as $a\angle{2}b$, $a\angle{3}b$, and $a\angle{4}b$.
Note that the functions $\log_a b$, and $\log^*_a b$ are not in the Coq Standard Library.
\end{rem}
\hide{
\begin{col}
	$\forall a \in \mathbb{N}$:
	\begin{enumerate}
		\item If $a\ge 1$, $\divc(a, b) = \left\lceil \frac{b}{a} \right\rceil$.
		\item If $a\ge 2$, $\logc(a, b) = \left\lceil \log_ab \right\rceil $ and $\logstarc(a, b) = \log^*_ab$.
	\end{enumerate}
\end{col}
\begin{proof}
	The result follows from \cref{col: inv-hyperop-234}, \cref{thm: inv-hyperop-correct} and the first few expansions of the hyperoperation hierarchy: $a[2]b = ab$, $a[3]b = a^b$ and $a[4]b = \ ^ba$.
\end{proof}

\begin{rem}
	\Cref{thm: cdt-recursion} leads to useful recursive formulas for $\divc$, $\logc$ and $\logstarc$:
	\begin{align*}
	\divc(a, b) & = 1 + \divc(a, b - a) & \text{ if } b > 0 &\text{, and } 0 \text{ otherwise}. \\
	\logc(a, b) & = 1 + \logc\left(a, \left\lceil b/a \right\rceil\right) & \text{ if } b > 1 &\text{, and } 0 \text{ otherwise}. \\
	\logstarc(a, b) & = 1 + \divc(a, \left\lceil \log_ab \right\rceil) & \text{ if } b > 1 &\text{, and } 0 \text{ otherwise}.
	\end{align*}
\end{rem}
}

\subsection{The inverse Ackermann hierarchy}

% NEW METHOD FOR INVERSE ACKERMANN
We want to use \emph{countdown} to build the \emph{inverse Ackermann hierarchy}, where each
level $\alpha_i$ inverts the level $\Ack_i$.
We know $\Ack_{i+1} = \rf{\Ack_i}{\Ack_i(1)}$, so the recursive
rule $\alpha_{i+1} \triangleq \cdt{\alpha_i}{\Ack_i(1)}$ is tempting.
But this approach is flawed because it still depends on $\Ack_i$.
Instead, we reexamine the inverse relationship: suppose $\alpha_i = \big(\Ack_i\big)^{-1}_+$ and $\alpha_{i+1} = \big(\Ack_{i+1}\big)^{-1}_+$. Then $\Ack_{i+1}(m) = \big(\Ack_{i}\big)^{(m)} \big(\Ack_{i}(1)\big)$. We then have:
\begin{equation} \label{eq: inv-ack-hier-derive}
\alpha_{i+1}(n)\le m \iff n\le \big(A_i\big)^{(m+1)}(1) \iff \big(\alpha_i\big)^{(m+1)}(n) \le 1
\end{equation}
Equivalently, $\alpha_{i+1}(n) = \min\big\{m : \big( \alpha_i \big)^{(m+1)}(n)\le 1\big\}$, or $\alpha_{i+1}(n) = \cdt{\alpha_i}{1}\big(\alpha_i(n)\big)$. From Equation \ref{eq: inv-ack-hier-derive} we can thus define the inverse Ackermann hierarchy:
\begin{defn} \label{defn: inv-ack-hier}
	$ \alpha_i \triangleq \begin{cases}
	\lambda n.(n - 1) & \text{if } i = 0
	\\ \big(\cdt{\alpha_{i-1}}{1}\big)\circ \alpha_{i-1} & \text{if } i\ge 1 \end{cases}
$
\end{defn}
Crucially, we have a new definition of $\alpha$ 
that is \emph{independent of $\Ack$}:
\begin{defn} \label{thm: inv-ack-hier-correct}
	%For all $n, k$, $n\le \Ack(k, k) \!\!\iff \!\! \alpha_k(n)\le k$. Thus
	$\alpha(n) \triangleq \min\big\{k : \alpha_k(n)\le k \big\}$.
\end{defn}
Finally, we must provide a structurally-recursive function that computes $\alpha$.
\begin{defn} \label{defn: inv-ack-worker}
	The inverse Ackermann worker is a function $\alpha^{\W}$: %(\mathbb{N}\to \mathbb{N}) \times \mathbb{N}^3\to \mathbb{N}$ such that for all $n, k, b\in \mathbb{N}$ and $f:\mathbb{N}\to \mathbb{N}$:
	\begin{equation} \label{eq: inv-ack-worker-recursion}
	\alpha^{\W}(f, n, k, b) = \begin{cases}
	k & \text{if } b = 0 \vee n\le k \\ \alpha^{\W}(\cdt{f}{1}\circ f , \cdt{f}{1}(n), k+1, b-1) & \text{if } b \ge 1 \wedge n \ge k+1
	\end{cases}
	\end{equation}
\end{defn}
%Given the arguments $\big(\alpha_i, \alpha_i(n), i, b\big)$ such that $\alpha_i(n) > i$ and $b > i$, $\alpha^{\W}$ takes on arguments $\big(\alpha_{i+1}, \alpha_{i+1}(n), i+1, b-1\big)$ at the next recursive call. Thus if $\alpha^{\W}$ is given a sufficient budget $b$, the initial arguments $(\alpha_0, \alpha_0(n), 0, b)$ will recursively move through the chain \note[what's with the braces?]{$\big\{\alpha_i(n)\big\}$} and terminate at a point $k$ where $\alpha_k(n)\le k$.
Given the arguments $\big(\alpha_i, \alpha_i(n), i, b - i\big)$ such that $\alpha_i(n) > i$ and $b > i$, $\alpha^{\W}$ takes on arguments $\big(\alpha_{i+1}, \alpha_{i+1}(n), i+1, b - (i+1)\big)$ at the next recursive call. Thus if $\alpha^{\W}$ is given a sufficient budget $b$, it will recursively transform the tuple $(\alpha_k, \alpha_k(n), k, b - k)$ until a point $k$ where $\alpha_k(n)\le k$, and will then return $k$.
We now need to show that $\alpha^{\W}$ can correctly compute $\alpha(n)$
given a reasonable budget. We show that a budget of $n$ suffices.
We start with the following lemma.
\begin{lem} \label{lem: inv-ack-worker-intermediate}
	$\forall n, b, k$ such that $k+1\le \min\big\{b, \alpha_k(n)\big\}$, 
	\begin{equation*}
	\alpha^{\W}\big(\alpha_0, \alpha_0(n), 0, b\big) = \alpha^{\W}\big(\alpha_{k+1}, \alpha_{k+1}(n), k+1, b-k-1\big)
	\end{equation*}
\end{lem}
\begin{proof}
	 We prove $P(k)$ by induction, where
	 \begin{equation*}
	 \begin{aligned}
	 P(k) \quad \triangleq \quad & (\alpha_k(n)\ge k+1) \wedge (b\ge k+1) \implies \null \\ & \alpha^{\W}\big(\alpha_0, \alpha_0(n), 0, b\big) = \alpha^{\W}\big(\alpha_{k+1}, \alpha_{k+1}(n), k+1, b-k-1\big)
	 \end{aligned}
	 \end{equation*}
	\begin{itemize}[leftmargin=*]
		\item \emph{Base case}. $\alpha^{\W}\big(\alpha_0, \alpha_0(n), 0, b\big) = \alpha^{\W}\big(\cdt{\big(\alpha_0}{1}\big)\circ \alpha_0, \cdt{\alpha_0}{1}\big(\alpha_0(n)\big), 1, b - 1\big) $ by
		(\ref{eq: inv-ack-worker-recursion}) with $b\ge 1$ and $\alpha_0(n)\le 1$.
		Definition~\ref{defn: inv-ack-hier} gives $\alpha_1 = \big(\cdt{\alpha_0}{1}\big) \circ \alpha_0$, so $P(0)$ holds.
		
		\item \emph{Inductive step.} Suppose $\alpha_{k+1}(n)\ge k+2$ and $b\ge k+2$. Then $\alpha_k(n)\ge k+1$ and $b\ge k+1$, so $P(k)$ applies. It suffices to show
		\begin{equation*}
		\alpha^{\W}\big(\alpha_{k+1}, \alpha_{k+1}(n), k+1, b-k-1\big)
		= \alpha^{\W}\big(\alpha_{k+2}, \alpha_{k+2}(n), k+2, b-k-2\big)
		\end{equation*}
		Definition~\ref{defn: inv-ack-hier} gives $\alpha_{k+2} = \big(\cdt{\alpha_{k+1}}{1}\big)\circ \alpha_{k+1}$, so this 
		is~(\ref{eq: inv-ack-worker-recursion}) with $b - k - 1\ge 1$ and $\alpha_{k+1}(n)\ge k+2$. Thus $P(k+1)$ holds. 
		%\vspace*{-\baselineskip}
	\end{itemize}
	% \vspace{-2.2em}
\end{proof}
\hide{\color{red}
\begin{proof}
	 We prove $P(k) \ \forall k$ by induction, where
	 \begin{equation*}
	 \begin{aligned}
	 P(k) \triangleq \forall n, b \ \ & (\alpha_k(n)\ge k+1) \to (b\ge k+1)\\ & \to \W\alpha\big(\alpha_0, \alpha_0(n), 0, b\big) = \W\alpha\big(\alpha_{k+1}, \alpha_{k+1}(n), k+1, b-k-1\big)
	 \end{aligned}
	 \end{equation*}
		\begin{itemize}[leftmargin=*]
		\item \emph{Base case}. $ \W\alpha\big(\alpha_0, \alpha_0(n), 0, b\big) = \W\alpha\big(\cdt{\big(\alpha_0}{1}\big)\circ \alpha_0, \cdt{\alpha_0}{1}\big(\alpha_0(n)\big), 1, b - 1\big) $ by
		\eqref{eq: inv-ack-worker-recursion} with $b\ge 1$ and $\alpha_0(n)\le 1$. Since $\alpha_1 = \big(\cdt{\alpha_0}{1}\big) \circ \alpha_0$ per Definition~\ref{defn: inv-ack-hier}, $P(0)$ holds.
		
		\item \emph{Inductive step.} Suppose $\alpha_{k+1}(n)\ge k+2$ and $b\ge k+2$. Then $\alpha_k(n)\ge k+1$ and $b\ge k+1$, so $P(k)$ applies. It suffices to show
		\begin{equation*}
		\W\alpha\big(\alpha_{k+1}, \alpha_{k+1}(n), k+1, b-k-1\big)
		= \W\alpha\big(\alpha_{k+2}, \alpha_{k+2}(n), k+2, b-k-2\big)
		\end{equation*}
		Per Definition~\ref{defn: inv-ack-hier}, $\alpha_{k+2} = \big(\cdt{\alpha_{k+1}}{1}\big)\circ \alpha_{k+1}$, so this is just \eqref{eq: inv-ack-worker-recursion} with $b - k - 1\ge 1$ and $\alpha_{k+1}(n)\ge k+2$, so $P(k+1)$ holds. The proof is complete by induction.\vspace*{-\baselineskip}
	\end{itemize}
\end{proof}}%end hide

\noindent We are finally ready for a strategy to compute the inverse Ackermann function:
%formalizes a setting for $\W\alpha$ to work.
\begin{thm} \label{thm: inv-ack-worker-correct}
	$\alpha^{\W}\big(\alpha_0, \alpha_0(n), 0, n\big) = \alpha(n)$.
\end{thm}



%Next, a lemma connecting the value of $\W\alpha(f, n, k , b)$ and $k$, which is important because the recursive rule alone does not tell how the value of $\W\alpha$ changes at each recursive step.
%\begin{lem}
%	For all $f, n, k, b$, $\W\alpha\big(f, n, k, b\big) \ge k$.
%\end{lem}
%\begin{proof}
%	Fix $n$, if $k \ge n$, equality occurs. Consider only $k\le n$, using backwards induction, suppose $\W\alpha\big(f, n, k, b\big) \ge k \ \forall f, b$ for some $1\le k\le n$. Now fix $f, b$ and consider $\W\alpha\big(f, n, k-1, b\big)$. If $b = 0$, equality occurs. Otherwise, $\W\alpha\big(f, n, k-1, b\big) = \W\alpha\big(f, n, k, b\big) \ge k \ge k-1$. The proof is complete.
%\end{proof}
\begin{proof} %[Proof of \Cref{thm: inv-ack-worker-correct}]
	Since the sequence $\big\{\alpha_k(n)\big\}_{k=1}^{\infty}$ decreases while $\{k\}_{k=1}^{\infty}$ increases to infinity, there exists $m \triangleq \min\big\{k : \alpha_k(n) \le k \} = \alpha(n)$. Note that $m\le n$ since $\alpha_n(n)\le n$.
	If $m = 0$, $\alpha_0(n)\le 0 \!\! \implies \!\! \alpha_0(n) = 0$. Thus $\alpha^{\W}\big(\alpha_0, \alpha_0(n), 0, n\big) = 0 = m$. If $m \ge 1$, Lemma~\ref{lem: inv-ack-worker-intermediate} implies:
	$$ \alpha^{\W}\big(\alpha_0, \alpha_0(n), 0, n\big) = \alpha^{\W}\big(\alpha_m, \alpha_m(n), m, n - m\big) = m $$
	where the last equality follows from the recursive rule.
\end{proof}
% The code to compute the inverse Ackermann function in Gallina follows.
\begin{lstlisting}
`\href{https://github.com/inv-ack/inv-ack/blob/6099297c6ab0e16d14b037fb5ed600c4d22818f6/inv_ack.v#L138-L148} {Fixpoint inv\_ack\_worker}` (f : nat -> nat) (n k b : nat) : nat :=
  match b with
  | 0 => 0
  | S b' => match (n - k) with
            | 0 => k
            | S _ =>
              let g := (countdown_to 1 f) in 
              inv_ack_worker (compose g f) (g n) (S k) b'
            end
  end.

`\href{https://github.com/inv-ack/inv-ack/blob/6099297c6ab0e16d14b037fb5ed600c4d22818f6/inv_ack.v#L32-L36}{Fixpoint alpha}` (m x : nat) : nat :=
  match m with
  | 0 => x - 1
  | S m' => countdown_to 1 (alpha m') (alpha m' x)
  end.
  
`\href{https://github.com/inv-ack/inv-ack/blob/6099297c6ab0e16d14b037fb5ed600c4d22818f6/inv_ack.v#L151-L152}{Definition inv\_ack}` (n : nat) : nat :=
  match (alpha 0) with f => inv_ack_worker f (f n) 0 n end.
\end{lstlisting}

% OLD METHOD FOR INVERSE ACKERMANN

%Using the Ackermann kludge from \cref{sec: overview}, we sketch a method to find the inverse Ackermann function from the inverse hyperoperations.
%\begin{thm} \label{thm: inv-hyperop-inv-ack}
%	For all $n, k$, $n\le \Ack(k, k) \iff 2\angle{k}(n+3)\le k+3$.
%\end{thm}
%\begin{proof}
%	$n\le \Ack(k, k) \iff n\le 2[k](k+3) - 3$. Now $2[k]$ is an expansion by \cref{thm: inv-hyperop-correct}'s proof, so $2[k](k+3) \ge k+3\ge 3$, so  $n\le 2[k](k+3) - 3 \iff n+3 \le 2[k](k+3)\iff 2\angle{k}(n+3)\le k+3$, again by \cref{thm: inv-hyperop-correct}.
%\end{proof}
%\Cref{thm: inv-hyperop-inv-ack} allows a simple method to compute the Inverse Ackermann function, based on the \emph{budget} idea in \emph{countdown worker}.
%\begin{defn} \label{defn: inv-ack-worker}
%	The \emph{inverse Ackermann worker} of $f$ is a function $\W\alpha\ : \mathbb{N}^4\to \mathbb{N}$ such that for all $n, k, b\in \mathbb{N}$ and $f:\mathbb{N}\to \mathbb{N}$:
%	$$ \W\alpha(f, n, k, b) = \begin{cases}
%	k - 3 & \text{if } b = 0 \vee f(n)\le k+3 \\ \W\alpha(\cdt{f}{a_k}\ , n, k+1, b-1) & \text{if } b \ge 1 \wedge f(n) > k+3
%	\end{cases} $$
%	where $a_0 = 2$, $a_1 = 0$ and $a_k = 1 \ \forall k\ge 2$.
%\end{defn}
%The function $\W\alpha$ takes a function $f$ and pretends it was the first level of the inverse hyperoperation hierarchy. It then keeps applying countdown to $f$, supposedly arrives at the $\text{m}^{\text{th}}$-level at the $\text{m}^{\text{th}}$-recursive step, until the budget $b$ is exhausted or $f(n)\le k+3$, i.e. \emph{early stopping}, and will output $k$. If at the beginning $k=3$ and $f = 2\angle{0}$, the early stopping condition becomes $2\angle{k}n \le k+3$, which when replace $n$ by $n+3$ gives what we need in \cref{thm: inv-hyperop-inv-ack}.
%The inverse Ackermann function can be defined as follows.
%\begin{thm} For all $n$, we have $\alpha(n) = \W\alpha(\lambda m.(m - 1), n+3, 3, n)$.
%\end{thm} 